cp

vale/code/arch/x64/interop/GenericInterop.fst
@@ -28,6 +28,12 @@ friend X64.Memory
 friend X64.Vale.Decls
 friend X64.Vale.StateLemmas
 
+////////////////////////////////////////////////////////////////////////////////
+// Vale-specific types supported by the interop layer
+//   Some integer types
+//   And arrays thereof
+////////////////////////////////////////////////////////////////////////////////
+
 type vale_type =
   | VT_Base of X64.Memory_s.base_typ
   | VT_Buffer of X64.Memory_s.base_typ
@@ -46,16 +52,34 @@ let vale_type_as_type : vale_type -> Type =
   | VT_Base bt -> base_type_as_type bt
   | VT_Buffer bt -> X64.Memory_s.buffer (TBase bt)
 
+
+////////////////////////////////////////////////////////////////////////////////
+// as_l/r_tuple: Interpreting a list of vale types as
+//               a left- or right-nested pair
+////////////////////////////////////////////////////////////////////////////////
+let rec as_right_tuple (dom:list vale_type{Cons? dom}) =
+  match dom with
+  | [x] -> vale_type_as_type x
+  | hd::tl -> vale_type_as_type hd & as_right_tuple tl
+
+let rec as_left_tuple (acc:Type) (dom:list vale_type)
+  : Tot Type (decreases dom) =
+  match dom with
+  | [] -> acc
+  | hd::tl -> as_left_tuple (acc & vale_type_as_type hd) tl
+
+////////////////////////////////////////////////////////////////////////////////
+// n_arrow: Arrows with a generic number of vale types as the domain
+//          and a result type `codom` that does not depend on the domain
+////////////////////////////////////////////////////////////////////////////////
 [@unifier_hint_injective]
 let rec n_arrow (dom:list vale_type) (codom:Type) =
   match dom with
   | [] -> codom
   | hd::tl -> vale_type_as_type hd -> n_arrow tl codom
 
-let rec as_tuple (dom:list vale_type{Cons? dom}) =
-  match dom with
-  | [x] -> vale_type_as_type x
-  | hd::tl -> vale_type_as_type hd & as_tuple tl
+[@unifier_hint_injective]
+let arr (dom:Type) (codom:Type) = dom -> codom
 
 let elim_1 (#dom:list vale_type{Cons? dom})
            (#r:Type)
@@ -69,26 +93,31 @@ let elim_nil (#dom:list vale_type{Nil? dom})
     : r =
     f
 
+let intro_n_arrow_nil (a:Type) (x:a)
+  : n_arrow [] a
+  = x
+
+let intro_n_arrow_cons (hd:vale_type) (b:Type) (tl:list vale_type)
+                       (x:vale_type_as_type hd -> n_arrow tl b)
+  : n_arrow (hd::tl) b
+  = x
+
+////////////////////////////////////////////////////////////////////////////////
+// n_dep_arrow: Arrows with a generic number of vale types as the domain
+//              and a result type codom that depends on the domain
+////////////////////////////////////////////////////////////////////////////////
 [@unifier_hint_injective]
 let rec n_dep_arrow (dom:list vale_type) (codom: n_arrow dom Type) =
   match dom with
   | [] -> codom
   | hd::tl -> x:vale_type_as_type hd -> n_dep_arrow tl (elim_1 codom x)
 
-let rec dom_as_tuple (acc:Type) (dom:list vale_type)
-  : Tot Type (decreases dom) =
-  match dom with
-  | [] -> acc
-  | hd::tl -> dom_as_tuple (acc & vale_type_as_type hd) tl
-
-[@unifier_hint_injective]
-let arr (dom:Type) (codom:Type) = dom -> codom
-
+//unused
 let rec n_dep_arrow_uncurry
         (prefix: Type)
         (v:prefix)
         (dom:list vale_type)
-        (codom: arr (dom_as_tuple prefix dom) Type)
+        (codom: arr (as_left_tuple prefix dom) Type)
   : Tot Type (decreases dom) =
   match dom with
   | [] -> codom v
@@ -99,99 +128,6 @@ let rec n_dep_arrow_uncurry
       (v, x)
       tl
       codom
-
-let vale_pre_tl (dom:list vale_type) =
-    n_arrow dom prop
-
-let vale_pre (dom:list vale_type) =
-    code:va_code ->
-    s0:va_state ->
-    win:bool ->
-    stack:buffer (TBase TUInt64) ->
-    vale_pre_tl dom
-
-let vale_post_tl (dom:list vale_type) =
-    n_arrow dom (s1:va_state -> f:va_fuel -> prop)
-
-let vale_post (dom:list vale_type) =
-    code:va_code ->
-    s0:va_state ->
-    win:bool ->
-    stack:buffer (TBase TUInt64) ->
-    vale_post_tl dom
-
-let rec vale_sig_tl (#dom:list vale_type{Cons? dom})
-                    (pre:vale_pre_tl dom)
-                    (post:vale_post_tl dom)
-  : Type =
-    match dom with
-    | [hd] ->
-      x:vale_type_as_type hd ->
-      Ghost (va_state & va_fuel)
-            (requires (elim_1 pre x))
-            (ensures (fun (s1, f) -> elim_nil (elim_1 post x) s1 f))
-    | hd::tl ->
-      x:vale_type_as_type hd ->
-      vale_sig_tl #tl (elim_1 pre x) (elim_1 post x)
-
-let vale_sig (#dom:list vale_type{Cons? dom})
-             (pre:vale_pre dom)
-             (post:vale_post dom)
-  : Type =
-    va_b0:va_code ->
-    va_s0:va_state ->
-    win:bool ->
-    stack_b:buffer64 ->
-    vale_sig_tl (pre va_b0 va_s0 win stack_b)
-                (post va_b0 va_s0 win stack_b)
-
-let rec create_buffer_list (dom:list vale_type) (acc:list b8)
-    : n_arrow dom (list b8) =
-    match dom with
-    | [] -> acc
-    | hd::tl ->
-      (fun (x:vale_type_as_type hd) -> create_buffer_list tl (if VT_Buffer? hd then x::acc else acc))
-
-
-// let create_buffer_list (dst:b8) (src:b8) (stack_b:b8)  : (l:list b8{
-//     l == [stack_b;dst;src] /\
-//   (forall x. {:pattern List.memP x l} List.memP x l <==> (x == dst \/ x == src \/ x == stack_b))}) =
-//   [stack_b;dst;src]
-let maybe_cons_buffer (a:vale_type) (x:vale_type_as_type a) (acc:list b8) : list b8 =
-  if VT_Buffer? a then x::acc else acc
-
-let rec initial_state_t
-              (dom:list vale_type)
-              (acc:list b8)
-              (codom:Type)
-  : n_arrow dom Type =
-    match dom with
-    | [] ->
-      (h0:HS.mem{ Interop.list_disjoint_or_eq acc /\
-                  Interop.list_live h0 acc } ->
-       GTot codom)
-    | hd::tl ->
-      fun (x:vale_type_as_type hd) ->
-         initial_state_t tl (maybe_cons_buffer hd x acc) codom
-
-let fold_initial_state_t
-  (#hd:vale_type) (#tl:list vale_type)
-  (#x:vale_type_as_type hd) (#acc:list b8) (#codom:Type)
-  (res:n_dep_arrow tl (initial_state_t tl (maybe_cons_buffer hd x acc) codom))
-  : n_dep_arrow tl (elim_1 (initial_state_t (hd::tl) acc codom) x)
-  = res
-
-let initial_trusted_state_t (dom:list vale_type) (acc:list b8) =
-  initial_state_t dom acc (TS.traceState & mem)
-
-let intro_n_arrow_nil (a:Type) (x:a)
-  : n_arrow [] a
-  = x
-
-let intro_n_arrow_cons (hd:vale_type) (b:Type) (tl:list vale_type)
-                       (x:vale_type_as_type hd -> n_arrow tl b)
-  : n_arrow (hd::tl) b
-  = x
 
 let intro_dep_arrow_nil (b:Type)
                         (f:b)
@@ -211,9 +147,72 @@ let intro_dep_arrow_cons (hd:vale_type)
   : n_dep_arrow (hd::tl) b
   = f
 
+let elim_dep_arrow_nil (#codom:n_arrow [] Type)
+                       (f:n_dep_arrow [] codom)
+    : elim_nil codom
+   = f
+
+let elim_dep_arrow_cons (hd:vale_type)
+                        (tl:list vale_type)
+                        (#codom:n_arrow (hd::tl) Type)
+                        (f:n_dep_arrow (hd::tl) codom)
+    : x:vale_type_as_type hd ->
+      n_dep_arrow tl (elim_1 codom x)
+   = f
+
+//Just a small test function to see how these coercions work
 let test : n_dep_arrow [VT_Base TUInt8] (fun (x:UInt8.t) -> y:UInt8.t{x == y}) =
   fun (x:UInt8.t) -> intro_dep_arrow_nil (y:UInt8.t{x == y}) x
 
+////////////////////////////////////////////////////////////////////////////////
+// Creating initial states
+// The punchline of this section is the `create_both_initial_states`,
+// an arity generic function that builds a trusted state `t:TS.state`
+// and a vale state `v:va_state` with a proof that `t == state_to_S v`
+////////////////////////////////////////////////////////////////////////////////
+let rec create_buffer_list (dom:list vale_type) (acc:list b8)
+    : n_arrow dom (list b8) =
+    match dom with
+    | [] -> acc
+    | hd::tl ->
+      (fun (x:vale_type_as_type hd) -> create_buffer_list tl (if VT_Buffer? hd then x::acc else acc))
+
+let maybe_cons_buffer (a:vale_type) (x:vale_type_as_type a) (acc:list b8) : list b8 =
+  if VT_Buffer? a then x::acc else acc
+
+
+let mem_roots (roots:list b8) =
+    h0:HS.mem{ Interop.list_disjoint_or_eq roots /\
+               Interop.list_live h0 roots }
+
+let rec initial_state_t
+              (dom:list vale_type)
+              (acc:list b8)
+              (codom:Type)
+  : n_arrow dom Type =
+    match dom with
+    | [] ->
+      (mem_roots acc ->
+       GTot codom)
+    | hd::tl ->
+      fun (x:vale_type_as_type hd) ->
+         initial_state_t tl (maybe_cons_buffer hd x acc) codom
+
+// Some identity coercions that serve as proof hints
+// to introduce generic arrow types
+let fold_initial_state_t
+  (#hd:vale_type) (#tl:list vale_type)
+  (#x:vale_type_as_type hd) (#acc:list b8) (#codom:Type)
+  (res:n_dep_arrow tl (initial_state_t tl (maybe_cons_buffer hd x acc) codom))
+  : n_dep_arrow tl (elim_1 (initial_state_t (hd::tl) acc codom) x)
+  = res
+
+let initial_trusted_state_t (dom:list vale_type) (acc:list b8) =
+  initial_state_t dom acc (TS.traceState & mem)
+
+////////////////////////////////////////////////////////////////////////////////
+//The calling convention w.r.t the register mapping
+////////////////////////////////////////////////////////////////////////////////
 let max_arity (is_win:bool) = if is_win then 4 else 6
 
 let register_of_arg_i (is_win:bool) (i:nat{i < max_arity is_win}) : reg =
@@ -232,6 +231,7 @@ let register_of_arg_i (is_win:bool) (i:nat{i < max_arity is_win}) : reg =
     | 4 -> R8
     | 5 -> R9
 
+//A partial inverse of the above function
 let arg_of_register (is_win:bool) (r:reg)
   : option (i:nat{i < max_arity is_win /\ register_of_arg_i is_win i = r})
   = if is_win then
@@ -270,8 +270,6 @@ let update_regs (#a:vale_type)
         UInt32.v x
       | VT_Base TUInt64 ->
         UInt64.v x
-      | VT_Base TUInt128 ->
-        0 //IMPOSSIBLE
       | VT_Buffer _ ->
         addrs x
     in
@@ -297,13 +295,15 @@ let update_taint_map (#a:vale_type)
         else taint y
     | _ -> taint
 
+// Splitting the construction of the initial state into two functions
+// one that creates the initial trusted state (i.e., part of our TCB)
+// and another that just creates the vale state, a view upon the trusted one
 let create_initial_trusted_state_core
        (acc:list b8)
        (regs:registers)
        (xmms:xmms_t)
        (taint:taint_map)
-       (h0:HS.mem{ Interop.list_disjoint_or_eq acc /\
-                   Interop.list_live h0 acc })
+       (h0:mem_roots acc)
   : GTot (TS.traceState & mem)
   = let (mem:mem) = {
       addrs = addrs;
@@ -326,10 +326,66 @@ let create_initial_trusted_state_core
     },
     mem
 
-let mem_roots (roots:list b8) =
-    h0:HS.mem{ Interop.list_disjoint_or_eq roots /\
-               Interop.list_live h0 roots }
 
+let initial_vale_state_t (dom:list vale_type) (acc:list b8) =
+  initial_state_t dom acc va_state
+
+let create_initial_vale_state_core
+       (acc:list b8)
+       (regs:registers)
+       (xmms:xmms_t)
+       (taint:taint_map)
+       (h0:mem_roots acc)
+  : GTot va_state
+  = let t_state, mem = create_initial_trusted_state_core acc regs xmms taint h0 in
+    {ok = TS.(BS.(t_state.state.ok));
+     regs = X64.Vale.Regs.of_fun TS.(BS.(t_state.state.regs));
+     xmms =  X64.Vale.Xmms.of_fun TS.(BS.(t_state.state.xmms));
+     flags = TS.(BS.(t_state.state.flags));
+     mem = mem;
+     memTaint = TS.(t_state.memTaint)}
+
+let core_create_lemma
+       (acc:list b8)
+       (regs:registers)
+       (xmms:xmms_t)
+       (taint:taint_map)
+       (h0:mem_roots acc)
+  : Lemma
+      (ensures (fst (create_initial_trusted_state_core acc regs xmms taint h0) ==
+                state_to_S (create_initial_vale_state_core acc regs xmms taint h0)))
+  = let s_init, _ = (create_initial_trusted_state_core acc regs xmms taint h0) in
+    let s0 = (create_initial_vale_state_core acc regs xmms taint h0) in
+    let s1 = state_to_S s0 in
+    assert (FunctionalExtensionality.feq (regs' s1.TS.state) (regs' s_init.TS.state));
+    assert (FunctionalExtensionality.feq (xmms' s1.TS.state) (xmms' s_init.TS.state))
+
+let create_both_initial_states_core
+       (acc:list b8)
+       (regs:registers)
+       (xmms:xmms_t)
+       (taint:taint_map)
+       (h0:HS.mem{ Interop.list_disjoint_or_eq acc /\
+                   Interop.list_live h0 acc })
+    : GTot (t:TS.traceState &
+            v:va_state{
+              t == state_to_S v
+            })
+    = let t, _ = create_initial_trusted_state_core acc regs xmms taint h0 in
+      let v = create_initial_vale_state_core acc regs xmms taint h0 in
+      core_create_lemma acc regs xmms taint h0;
+      (|t, v|)
+
+//The type of an arity-generic function that produces a pair
+//of related trusted and vale states
+let both_initial_states_t (dom:list vale_type) (acc:list b8) =
+  initial_state_t dom acc (t:TS.traceState & v:va_state{t == state_to_S v})
+
+//This function folds over the `dom:list vale_type`
+//and builds an arity-generic dependent function that constructs
+//the initial states
+//It's maybe more generic than it needs to be, since it is now applied only
+//once, i.e., with f = create_both_initial_states
 let rec create_initial_state_aux
         #codom
         (dom:list vale_type)
@@ -379,13 +435,13 @@ let init_regs (stack_b:b8) : registers =
         addrs stack_b
       else init_regs r
 
-let create_initial_trusted_state
+let create_both_initial_states
       (is_win:bool)
       (stack_b:b8)
       (dom:list vale_type{List.length dom < max_arity is_win})
     : n_dep_arrow
          dom
-         (initial_trusted_state_t dom [stack_b])
+         (both_initial_states_t dom [stack_b])
     = create_initial_state_aux
           dom
           is_win
@@ -394,55 +450,144 @@ let create_initial_trusted_state
           init_xmms
           [stack_b]
           init_taint
-          create_initial_trusted_state_core
+          create_both_initial_states_core
 
-let initial_vale_state_t (dom:list vale_type) (acc:list b8) =
-  initial_state_t dom acc va_state
+let create_vale_initial_state_t (dom:list vale_type)
+                                (acc:list b8)
+    = n_dep_arrow
+          dom
+          (initial_vale_state_t dom acc)
 
-let create_initial_vale_state_core
-       (acc:list b8)
-       (regs:registers)
-       (xmms:xmms_t)
-       (taint:taint_map)
-       (h0:HS.mem{ Interop.list_disjoint_or_eq acc /\
-                   Interop.list_live h0 acc })
-  : GTot va_state
-  = let t_state, mem = create_initial_trusted_state_core acc regs xmms taint h0 in
-    {ok = TS.(BS.(t_state.state.ok));
-     regs = X64.Vale.Regs.of_fun TS.(BS.(t_state.state.regs));
-     xmms =  X64.Vale.Xmms.of_fun TS.(BS.(t_state.state.xmms));
-     flags = TS.(BS.(t_state.state.flags));
-     mem = mem;
-     memTaint = TS.(t_state.memTaint)}
+let create_vale_initial_state (dom:list vale_type{List.length dom < max_arity win})
+                              (acc:list b8)
+  : create_vale_initial_state_t dom
+                                acc
+  = create_initial_state_aux
+          dom
+          win
+          0
+          Interop_assumptions.init_regs
+          init_xmms
+          acc
+          init_taint
+          create_initial_vale_state_core
 
-let create_initial_vale_state
-       (is_win:bool)
-       (stack_b:b8)
-       (dom:list vale_type{List.length dom < max_arity is_win})
-    : n_dep_arrow
-         dom
-         (initial_vale_state_t dom [stack_b])
-     = create_initial_state_aux
-           dom
-           is_win
-           0
-           (init_regs stack_b)
-           init_xmms
-           [stack_b]
-           init_taint
-           create_initial_vale_state_core
+//////////////////////////////////////////////////////////////////////////////////////////
+//vale_sig pre post: a template for a top-level signature provided by a vale function
+//////////////////////////////////////////////////////////////////////////////////////////
+let stack_buffer = buffer (TBase TUInt64)
 
-let core_create_lemma
-       (acc:list b8)
-       (regs:registers)
-       (xmms:xmms_t)
-       (taint:taint_map)
-       (h0:mem_roots acc)
-  : Lemma
-      (ensures (fst (create_initial_trusted_state_core acc regs xmms taint h0) ==
-                state_to_S (create_initial_vale_state_core acc regs xmms taint h0)))
-  = let s_init, _ = (create_initial_trusted_state_core acc regs xmms taint h0) in
-    let s0 = (create_initial_vale_state_core acc regs xmms taint h0) in
-    let s1 = state_to_S s0 in
-    assert (FunctionalExtensionality.feq (regs' s1.TS.state) (regs' s_init.TS.state));
-    assert (FunctionalExtensionality.feq (xmms' s1.TS.state) (xmms' s_init.TS.state))
+let vale_pre_tl (dom:list vale_type) =
+    n_arrow dom (va_state -> stack_buffer -> prop)
+
+let vale_pre (dom:list vale_type) =
+    code:va_code ->
+    win:bool ->
+    vale_pre_tl dom
+
+let vale_post_tl (dom:list vale_type) =
+    n_arrow dom
+            (s0:va_state -> sb:stack_buffer -> s1:va_state -> f:va_fuel -> prop)
+
+let vale_post (dom:list vale_type) =
+    code:va_code ->
+    win:bool ->
+    vale_post_tl dom
+
+let rec vale_sig_tl (#dom:list vale_type)
+                    (pre:vale_pre_tl dom)
+                    (post:vale_post_tl dom)
+  : Type =
+    match dom with
+    | [] ->
+      va_s0:va_state ->
+      stack_b:stack_buffer ->
+      Ghost (va_state & va_fuel)
+            (requires (elim_nil pre va_s0 stack_b))
+            (ensures (fun (va_s1, f) -> elim_nil post va_s0 stack_b va_s1 f))
+
+    | hd::tl ->
+      x:vale_type_as_type hd ->
+      vale_sig_tl #tl (elim_1 pre x) (elim_1 post x)
+
+let vale_sig (#dom:list vale_type)
+             (pre:vale_pre dom)
+             (post:vale_post dom)
+  : Type =
+    va_b0:va_code ->
+    win:bool ->
+    vale_sig_tl (pre va_b0 win)
+                (post va_b0 win)
+
+//////////////////////////////////////////////////////////////////////////////////////////
+//lowstar_sig pre post:
+//    Interepreting a vale pre/post as a Low* function type
+//////////////////////////////////////////////////////////////////////////////////////////
+
+let mem_roots_p (h0:HS.mem) (roots:list b8) =
+  Interop.list_disjoint_or_eq roots /\
+  Interop.list_live h0 roots
+
+let elim_down_1 (hd:vale_type)
+                (acc:list b8)
+                (down:create_vale_initial_state_t [hd] acc)
+                (x:vale_type_as_type hd)
+    : mem_roots (maybe_cons_buffer hd x acc) -> GTot va_state =
+  let f : n_dep_arrow [] (elim_1 (initial_vale_state_t [hd] acc) x) = elim_dep_arrow_cons hd [] down x in
+  let g : (elim_1 (initial_vale_state_t [hd] acc) x) = elim_dep_arrow_nil f in
+  let h : (elim_1 (initial_state_t [hd] acc va_state) x) = g in
+  let i : (initial_state_t [] (maybe_cons_buffer hd x acc) va_state) = h in
+  i
+
+let elim_down_cons (hd:vale_type)
+                   (tl:list vale_type)
+                   (acc:list b8)
+                   (down:create_vale_initial_state_t (hd::tl) acc)
+                   (x:vale_type_as_type hd)
+    : create_vale_initial_state_t tl (maybe_cons_buffer hd x acc) =
+    elim_dep_arrow_cons hd tl down x
+
+let rec as_lowstar_sig_tl (#dom:list vale_type{Cons? dom})
+                          (acc:list b8)
+                          (down:create_vale_initial_state_t dom acc)
+                          (pre: vale_pre_tl dom)
+                          (post: vale_post_tl dom)
+    : Type =
+    match dom with
+    | [hd] ->
+      x:vale_type_as_type hd ->
+      Stack unit
+        (requires (fun h0 ->
+                    let acc1 = maybe_cons_buffer hd x acc in
+                    mem_roots_p h0 acc1 /\
+                    (forall (h0':mem_roots acc1)
+                       (b:stack_buffer)
+                       (v:va_state).
+                            HS.fresh_frame h0 h0' /\
+                            B.frameOf b == HS.get_tip h0' /\
+                            B.live h0' b /\ //some trouble here with b not being in acc
+                            v == elim_down_1 hd acc down x h0' ==>
+                            elim_nil (elim_1 pre x) v b)))
+        (ensures (fun h0 _ h1 -> True))
+
+    | hd::tl ->
+      x:vale_type_as_type hd ->
+      as_lowstar_sig_tl
+        #tl
+        (maybe_cons_buffer hd x acc)
+        (elim_down_cons hd tl acc down x)
+        (elim_1 pre x)
+        (elim_1 post x)
+
+let as_lowstar_sig  (#dom:list vale_type{Cons? dom /\ List.length dom < max_arity win})
+                    (pre: vale_pre dom)
+                    (post: vale_post dom) =
+    va_b0:va_code ->
+    as_lowstar_sig_tl
+      #dom
+      []
+      (create_vale_initial_state dom [])
+      (pre va_b0 win)
+      (post va_b0 win)
+
+////////////////////////////////////////////////////////////////////////////////
